Set-up for extraction; some boilerplate code in thermostat replaced with more generic tactics
Ignore-this: 6b5ccc87f72656af0d325b3ba3a43741

darcs-hash:20090517104327-20b81-f6236f8ba2a7e3f5285ca3532f4c1de7e5802c74.gz

thermostat_test.ml
@@ -1,0 +1,1 @@
+let _ = Printf.printf "Thermostat unsafe=%b\n" Thermostat_patched.unsafe
