hs_solver.v
@@ -1,0 +1,166 @@
+Require Import geometry.
+Require Export Program.
+Require Import EquivDec.
+Require square_abstraction.
+
+Open Local Scope CR_scope.
+
+Hint Unfold in_orange orange_left orange_right : hybsys.
+
+Hint Rewrite CRplus_Qplus CRminus_Qminus CRopp_Qopp 
+  CRmult_Qmult CRinv_Qinv : CR_Q.
+
+Ltac CR_Q_pre := autorewrite with CR_Q.
+
+Ltac CRcmp_to_O :=
+  let go x :=
+    exists x%Qpos; ring_simplify; vm_compute; intros; discriminate
+  in
+  match goal with
+  | |- '0 < '?x =>
+      match type of x with
+      | Q => 
+          match eval compute in (Qnum x) with
+          | Zpos ?v => go (v # Qden x)%Qpos
+          end
+      | positive => go x
+      | nat => go (P_of_succ_nat (x - 1))
+      end
+  end.
+
+Ltac prove_NoDup := simpl;
+  match goal with
+  | |- NoDup [] => constructor 1
+  | |- NoDup _ => constructor 2; [vm_compute; intuition; discriminate | prove_NoDup ]
+  end.
+
+Ltac prove_exhaustive_list :=
+  destruct 0; vm_compute; tauto.
+
+Ltac wd_helper :=
+  match goal with
+  | H: regFunEq ?x ?y |- 
+    `match CR_le_le_dec ?x ?v with
+    | left _ => _ | right _ => _
+     end
+    =
+    `match CR_le_le_dec ?y ?v' with
+    | left _ => _ | right _ => _
+     end =>
+    let e := fresh "e" in
+    set (e := @CR_le_le_dec_wd _ _ v v H (genericSetoid_Reflexive _ _)); clearbody e;
+    destruct (CR_le_le_dec x v) in *; 
+    destruct (CR_le_le_dec y v) in *; 
+    auto; try discriminate; clear e
+  end.
+
+Ltac qrange := unfold uncurry; vm_compute; intuition; discriminate.
+
+Ltac equiv_dec := repeat intro; 
+  match goal with
+  | |- {Equivalence.equiv ?x ?y} + {_} =>
+    cut (decision (x = y)); [auto | dec_eq]
+  end.
+
+Ltac decomp_hyp H := 
+  match type of H with
+  | _ /\ _ => decompose [Logic.and] H; clear H
+  | _ \/ _ => decompose [Logic.or] H; clear H
+  | ex _ => decompose [ex] H; clear H
+  | sig _ => decompose record H; clear H
+  end.
+
+Ltac decomp :=
+  repeat
+    match goal with
+    | H: _ |- _ => decomp_hyp H
+    end.
+
+Ltac destruct_hs_data :=
+  repeat
+    match goal with
+    | H: ?x * ?y |- _ => destruct H; clear H
+    | p : Point |- _ => destruct p; clear p
+    end.
+
+Ltac simplify_hyps :=
+  intros;
+  repeat progress 
+    (destruct_hs_data; 
+     decomp;
+     try subst; 
+     simpl in *).
+
+Ltac full_split :=
+  repeat 
+    match goal with
+    | |- ?x /\ ?y => split
+    | |- ?x <-> ?y => split; simplify_hyps; intros
+    end.
+
+Ltac single_rewrite :=
+  match goal with
+  | H: _ |- _ => rewrite H; clear H
+  | H: _ |- _ => rewrite <- H; clear H
+  end.
+
+Ltac esubst :=
+  repeat single_rewrite; try subst.
+
+Ltac simplify_proj :=
+  repeat
+    match goal with
+    | |- context [`?x] => destruct x; simpl
+    end.
+
+Ltac hs_unfolds := 
+  repeat progress (
+    unfold 
+      Basics.compose,
+      in_orange, in_osquare, orange_left, orange_right,
+      square_abstraction.in_region,
+      square_abstraction.absInterval;
+    simpl).
+
+Ltac CRle_solve :=
+  match goal with
+  | H: ?x <= ?y |- _ <= ?y =>
+      solve [apply CRle_trans with x; auto || CRle_constants]
+  | H: ?x <= ?y |- ?x <= _ =>
+      solve [apply CRle_trans with y; auto || CRle_constants]
+  | _ => solve [CRle_constants]
+  end.
+
+Ltac grind tac := 
+  match goal with
+  | |- '0 < '_ => CRcmp_to_O
+  | |- forall x, In x _ => 
+      prove_exhaustive_list
+  | |- _ =>
+    hs_unfolds; intros; simpl;
+    try solve [intros; CRle_constants | program_simplify | auto with hybsys];
+      match goal with
+      | |- uncurry Qle _ =>
+          qrange
+      | |- OQle _ =>
+          qrange
+      | H: regFunEq ?x ?y |- `_ = `_ =>
+          repeat wd_helper
+      | |- NoDup _ =>
+          prove_NoDup
+      | |- EquivDec.EqDec _ _ =>
+          equiv_dec
+      | |- _ <= _ =>
+          CRle_solve
+      | |- _ =>
+          progress (
+            hs_unfolds; intros; simplify_hyps; 
+              full_split; esubst; eauto with hybsys; try tac
+          );
+          grind tac
+      end
+  end.
+
+Ltac hs_solver := grind idtac.
+
+Obligation Tactic := solve [hs_solver].
