thermostat_extract.v
@@ -1,0 +1,6 @@
+Require thermostat.
+
+Extract Inductive unit => "unit" [ "()" ].
+Extract Inductive bool => "bool" [ "true" "false" ].
+Extract Inductive sumbool => "bool" [ "true" "false" ].
+Extraction "thermostat" thermostat.unsafe.
