Makefile
@@ -1,0 +1,58 @@
+SHELL := /bin/sh
+
+MAKEFLAGS := -r -j
+
+.SUFFIXES:
+
+.PHONY: clean all config dist doc install-dist install-doc tags
+
+CoRN := /home/koper/CoRN
+CoLoR := /home/koper/color/color/
+COQMAKE := $(MAKE) -f Makefile.coq
+EXAMPLES := thermostat
+EXAMPLES_BIN := $(addsuffix .bin,$(EXAMPLES))
+EXAMPLES_GENERATED := $(addsuffix .ml,$(EXAMPLES)) $(addsuffix .mli,$(EXAMPLES))
+
+all: Makefile.coq
+	$(COQMAKE) OTHERFLAGS="-dont-load-proofs"
+
+Makefile.coq:
+	$(MAKE) config
+
+examples: $(EXAMPLES_BIN)
+
+%.bin: %_extract.vo
+	sed "s/failwith/fun _ -> failwith/" $*.ml > $*_patched.ml
+	ocamlopt $*.mli $*_patched.ml $*_test.ml -o $@
+	
+config:
+	$(COQBIN)/coq_makefile -R . HS -R $(CoRN) CoRN -R $(CoLoR) CoLoR `find ./*.v` > Makefile.coq
+	$(COQMAKE) depend
+
+clean:
+	rm -f *~ doc/HybSys.*.html doc/index.html $(EXAMPLES_GENERATED)
+	$(COQMAKE) clean
+
+tags:
+	$(COQBIN)/coqtags `find . -name \*.v`
+
+doc:
+	$(COQBIN)/coqdoc --html -g -d doc -R $(CoRN) CoRN -R $(CoLoR) CoLoR `find ./*.v`
+	./createIndex
+
+install-doc:
+	rm -rf $(WEB)/doc
+	mkdir $(WEB)/doc
+	cp doc/*.html doc/coqdoc.css $(WEB)/doc
+
+dist:
+	./createDist
+
+install-dist:
+	mv -f HybSys_`date +%y%m%d`.tar.gz $(WEB)/HybSys.tar.gz
+
+%.vo: %.v
+	$(COQMAKE) OTHERFLAGS="-dont-load-proofs" $@
+
+%:
+	$(COQMAKE) OTHERFLAGS="-dont-load-proofs" $@
